work towards approx

Denote/PCF/Approx.lean
@@ -1,16 +1,124 @@
 import Denote.PCF.Red
 import Denote.PCF.Denote
+import Denote.Domain.Scott
 
 namespace PCF
 
-def Approx : {t : Ty} → t.denote → ITerm [] t → Prop
+def ITerm.Approx : {t : Ty} → t.denote → ITerm [] t → Prop
   | .bool, .bot, _ | .nat, .bot, _ => True
   | .nat, .obj n, t => Red t (.ofNat n)
   | .bool, .obj .true, t => Red t .true
   | .bool, .obj .false, t => Red t .false
   | .arr _ _, d, t => ∀ e u, Approx e u → Approx (d.f (e)) (.app t u)
 
+def CtxApprox : {Γ : _} → ctx_denote Γ → (HList (ITerm []) Γ) → Prop
+  | [], .unit, .nil => True
+  | _ :: _, ⟨td, hd⟩, .cons ht tt => ht.Approx hd ∧ CtxApprox td tt
 
+namespace ITerm.Approx
+
+def bot : {t : _} → {e : ITerm [] t} → ITerm.Approx ⊥ e
+  | .nat, _ => .intro
+  | .bool, _ => .intro
+  | .arr _ _, _ => fun _ _ _ => bot
+
+theorem le_respects
+    : {t : _}
+    → {d' d : t.denote}
+    → {e : ITerm [] t}
+    → d' ≤ d
+    → ITerm.Approx d e
+    → ITerm.Approx d' e
+  | .nat, .obj _, .obj _, _, .obj_obj, h
+  | .bool, .obj _, .obj _, _, .obj_obj, h => h
+  | .bool, .bot, .bot, _, .bot_bot, _
+  | .bool, .bot, .obj _, _, .bot_obj, _
+  | .nat, .bot, .bot, _, .bot_bot, _
+  | .nat, .bot, .obj _, _, .bot_obj, _ => .bot
+  | .arr _ _, _, _, _, le, h => fun dx' dx v =>
+      le_respects (le dx') (h dx' dx v)
+
+theorem red_respects
+    : {t : _}
+    → {d : t.denote}
+    → {e e' : ITerm [] t}
+    → (∀ v, Red e v → Red e' v)
+    → ITerm.Approx d e
+    → ITerm.Approx d e'
+  | .bool, .bot, _, _, map, _
+  | .nat, .bot, _, _, map, _ => .bot
+  | .bool, .obj .true, _, _, map, h
+  | .bool, .obj .false, _, _, map, h
+  | .nat, .obj _, _, _, map, h => map _ h
+  | .arr Dom Ren, d, e, e', map, h =>
+    fun d' ex h' => red_respects (by
+        intro v h
+        rcases h with ((_|_)|_)
+        rename_i f h h'
+        refine .app (map _ h) h'
+      ) (h d' ex h')
+
+#check Dom.Ccss
+
+end ITerm.Approx
+
+open Dom in
+theorem fund : (e : ITerm Γ t) → (ρ σ : _) → CtxApprox ρ σ → (e.parSubst σ).Approx (e.denote ρ)
+  | .false, _, _, _ | .true, _, _, _ | .zero, _, _,_ => by
+    dsimp [ITerm.Approx, ITerm.denote, CFunc.const, ITerm.parSubst]
+    apply Red.val
+    grind
+  | .var _, _, _, _=> sorry
+  | .fix _, _, _, _ => sorry
+  | .z? e, ctx, _, h => by 
+    dsimp [z?.denote, CFunc.comp, ITerm.Approx, ITerm.denote, CFunc.const, ITerm.parSubst]
+    have := fund e ‹_› ‹_› h
+    generalize e.denote.f ctx = v at this
+    rcases v with (_|(_|⟨w⟩))
+    <;> dsimp [ITerm.Approx] at this
+    · exact .bot
+    · exact Red.z?z this
+    · exact Red.z?s this
+  | .pred e, ctx, _, h => by
+    dsimp [pred.denote, CFunc.comp, ITerm.Approx, ITerm.denote, CFunc.const, ITerm.parSubst]
+    have := fund e ‹_› ‹_› h
+    generalize e.denote.f ctx = v at this
+    rcases v with (_|(_|⟨v⟩))
+    any_goals exact .bot
+    exact Red.pred this
+  | .succ e, ctx, _, h => by
+    dsimp [succ.denote, CFunc.comp, ITerm.Approx, ITerm.denote, CFunc.const, ITerm.parSubst]
+    have := fund e ‹_› ‹_› h
+    generalize e.denote.f ctx = v at this
+    cases v
+    · exact .bot
+    · exact Red.succ this
+  | .ite e _ _, ctx, _, h => by
+    dsimp [Prod.corec, CFunc.corecP, ite.denote, CFunc.comp, ITerm.Approx, ITerm.denote, CFunc.const, ITerm.parSubst]
+    have := fund e ‹_› ‹_› h
+    generalize e.denote.f ctx = v at this
+    rcases v with (_|_|_)
+    <;> dsimp [ITerm.Approx, ite.denote'] at this ⊢
+    · exact .bot
+    · unfold ITerm.Approx
+      sorry
+    · sorry
+  | .app _ _, _, _, _ => sorry
+  | .lam _, _, _, _ => sorry
+
+theorem adeq_n {t : ITerm [] .nat}
+    (h : t.denote .unit = (ITerm.ofNat (Γ := []) n).denote .unit)
+    : Red t (ITerm.ofNat n) := by
+  have := fund t .unit .nil .intro
+  simpa [h, ITerm.ofNat_denote, ITerm.parSubst.closed, Dom.CFunc.const, ITerm.Approx] using this
+
+theorem adeq_b {t : ITerm [] .bool}
+    (h : t.denote .unit = (ITerm.ofBool (Γ := []) n).denote .unit)
+    : Red t (ITerm.ofBool n) := by
+  have := fund t .unit .nil .intro
+  cases n <;>
+  simpa [h, ITerm.ofBool_denote, ITerm.parSubst.closed, Dom.CFunc.const, ITerm.Approx] using this
 
 end PCF
+
 
